Src/Problem32.lean
@@ -7,17 +7,13 @@
 #check Nat.gcd
 
 /-- Euclidean algorithm -/
-def gcd (m n : Nat) : Nat :=
+partial def gcd (m n : Nat) : Nat :=
   -- sorry
   if m = 0 then
     n
   else
     gcd (n % m) m
   -- sorry
-
-  -- Avoid proving that the function terminates as a recursive function.
-  -- You don't have to fill in the `sorry` here.
-  decreasing_by sorry
 
 -- The following codes are for test and you should not edit these.
 
